more refactoring of BtreeSpec

examples/BtreeSpec.dfy
@@ -18,11 +18,11 @@ abstract module BtreeSpec {
     | Leaf(keys: seq<Key>, values: seq<Value>)
     | Index(pivots: seq<Key>, children: seq<Node>)
 
-  function LocalKeys(node: Node) : set<Key>
+  function PotentialPivots(node: Node) : set<Key>
   {
     match node {
-      case Leaf(keys, values) => set k | k in keys
-      case Index(pivots, children) => set k | k in pivots
+      case Leaf(keys, values) => set i | 0 < i < |keys| :: keys[i]
+      case Index(pivots, children) => set i | 0 <= i < |pivots| :: pivots[i]
     }    
   }    
     
@@ -44,9 +44,8 @@ abstract module BtreeSpec {
       && |node.pivots| == |node.children| - 1
       && Keys.IsStrictlySorted(node.pivots)
       && (forall i :: 0 <= i < |node.children| ==> WF(node.children[i]))
-      && (forall i :: 0 <= i < |node.children| ==> LocalKeys(node.children[i]) != {})
-      && (forall i, key :: 0 <= i < |node.children|-1 && key in LocalKeys(node.children[i]) ==> Keys.lt(key, node.pivots[i]))
-      && (forall i, key :: 0 < i < |node.children|   && key in LocalKeys(node.children[i]) ==> Keys.lte(node.pivots[i-1], key))
+      && (forall i, key :: 0 <= i < |node.children|-1 && key in PotentialPivots(node.children[i]) ==> Keys.lt(key, node.pivots[i]))
+      && (forall i, key :: 0 < i < |node.children|   && key in PotentialPivots(node.children[i]) ==> Keys.lt(node.pivots[i-1], key))
   }
 
   function Interpretation(node: Node) : map<Key, Value>
@@ -91,19 +90,30 @@ abstract module BtreeSpec {
     && oldleaf.Leaf?
     && leftleaf.Leaf?
     && rightleaf.Leaf?
-    && WF(oldleaf)
-    && WF(leftleaf)
-    && WF(rightleaf)
-    && 0 < |leftleaf.keys|
-    && 0 < |rightleaf.keys|
+    && 0 < |leftleaf.keys| == |leftleaf.values|
+    && 0 < |rightleaf.keys| == |rightleaf.values|
     && oldleaf.keys == leftleaf.keys + rightleaf.keys
     && oldleaf.values == leftleaf.values + rightleaf.values
-    && Keys.lt(Last(leftleaf.keys), pivot)
-    && Keys.lte(pivot, rightleaf.keys[0])
+    && pivot == rightleaf.keys[0]
+  }
+
+  lemma SplitLeafPreservesWF(oldleaf: Node, leftleaf: Node, rightleaf: Node, pivot: Key)
+    requires WF(oldleaf)
+    requires SplitLeaf(oldleaf, leftleaf, rightleaf, pivot)
+    ensures WF(leftleaf)
+    ensures WF(rightleaf)
+  {
+    Keys.StrictlySortedSubsequence(oldleaf.keys, 0, |leftleaf.keys|);
+    Keys.StrictlySortedSubsequence(oldleaf.keys, |leftleaf.keys|, |oldleaf.keys|);
+    assert Keys.IsStrictlySorted(oldleaf.keys[|leftleaf.keys|..|oldleaf.keys|]);
+    assert rightleaf.keys == oldleaf.keys[|leftleaf.keys|..|oldleaf.keys|];
   }
 
   lemma SplitLeafInterpretation(oldleaf: Node, leftleaf: Node, rightleaf: Node, pivot: Key)
     requires SplitLeaf(oldleaf, leftleaf, rightleaf, pivot)
+    requires WF(oldleaf)
+    requires WF(leftleaf)
+    requires WF(rightleaf)
     ensures Interpretation(oldleaf) == Keys.MapPivotedUnion(Interpretation(leftleaf), pivot, Interpretation(rightleaf))
   {
     var oldint := Interpretation(oldleaf);
@@ -112,14 +122,30 @@ abstract module BtreeSpec {
     var newint := Keys.MapPivotedUnion(leftint, pivot, rightint);
 
     forall key | key in oldint
-      ensures newint[key] == oldint[key]
+      ensures key in newint && newint[key] == oldint[key]
     {
       var llte := Keys.LargestLte(oldleaf.keys, key);
       if llte < |leftleaf.keys| {
         Keys.PosEqLargestLte(leftleaf.keys, key, llte);
+        Keys.IsStrictlySortedImpliesLt(oldleaf.keys, llte, |leftleaf.keys|);
       } else {
         var rightllte := llte - |leftleaf.keys|;
         Keys.PosEqLargestLte(rightleaf.keys, key, rightllte);
+        if |leftleaf.keys| < llte {
+          Keys.IsStrictlySortedImpliesLt(oldleaf.keys, |leftleaf.keys|, llte);
+        }
+      }
+    }
+
+    forall key | key in newint
+      ensures key in oldint && oldint[key] == newint[key]
+    {
+      if Keys.lt(key, pivot) {
+        var llte := Keys.LargestLte(leftleaf.keys, key);
+        Keys.PosEqLargestLte(oldleaf.keys, key, llte);
+      } else {
+        var llte := Keys.LargestLte(rightleaf.keys, key);
+        Keys.PosEqLargestLte(oldleaf.keys, key, |leftleaf.keys| + llte);
       }
     }
   }
@@ -132,7 +158,7 @@ abstract module BtreeSpec {
     Index(node.pivots[from..to-1], node.children[from..to])
   }
 
-  lemma WFSubIndexWF(node: Node, from: int, to: int)
+  lemma SubIndexPreservesWF(node: Node, from: int, to: int)
     requires WF(node)
     requires node.Index?
     requires 0 <= from < to <= |node.children|
@@ -147,16 +173,25 @@ abstract module BtreeSpec {
     && leftindex.Index?
     && rightindex.Index?
     && WF(oldindex)
-    && WF(leftindex)
-    && WF(rightindex)
     && 0 < |leftindex.children| < |oldindex.children|-1
     && leftindex == SubIndex(oldindex, 0, |leftindex.children|)
     && rightindex == SubIndex(oldindex, |leftindex.children|, |oldindex.children|)
     && pivot == oldindex.pivots[|leftindex.pivots|]
   }
 
+  lemma SplitIndexPreservesWF(oldindex: Node, leftindex: Node, rightindex: Node, pivot: Key)
+    requires SplitIndex(oldindex, leftindex, rightindex, pivot)
+    ensures WF(leftindex)
+    ensures WF(rightindex)
+  {
+    SubIndexPreservesWF(oldindex, 0, |leftindex.children|);
+    SubIndexPreservesWF(oldindex, |leftindex.children|, |oldindex.children|);
+  }
+  
   lemma SplitIndexInterpretation(oldindex: Node, leftindex: Node, rightindex: Node, pivot: Key)
     requires SplitIndex(oldindex, leftindex, rightindex, pivot)
+    requires WF(leftindex)
+    requires WF(rightindex)
     ensures Interpretation(oldindex) == Keys.MapPivotedUnion(Interpretation(leftindex), pivot, Interpretation(rightindex))
   {
     var oldint := Interpretation(oldindex);
@@ -172,26 +207,26 @@ abstract module BtreeSpec {
       AllKeysIsConsistentWithInterpretation(oldindex, key);
       var llte := Keys.LargestLte(oldindex.pivots, key);
       if Keys.lt(key, pivot) { 
-        assert llte < |leftindex.pivots|;
-        assert llte == Keys.LargestLte(leftindex.pivots, key);
-        assert key in Interpretation(oldindex.children[llte+1]);
-        assert oldint[key] == Interpretation(oldindex.children[llte+1])[key];
+        Keys.LargestLteSubsequence(oldindex.pivots, key, 0, |leftindex.pivots|);
         assert leftindex.children[llte+1] == oldindex.children[llte+1];
       } else {
+        Keys.LargestLteSubsequence(oldindex.pivots, key, |leftindex.pivots|+1, |oldindex.pivots|);
         assert rightindex.children[llte - |leftindex.children| + 1] == oldindex.children[llte + 1];
       }
     }
 
     forall key | key in newint
-      ensures MapsTo(oldint, key, newint[key])
+      ensures key in oldint
     {
       if Keys.lt(key, pivot) {
         AllKeysIsConsistentWithInterpretation(leftindex, key);
         var llte := Keys.LargestLte(leftindex.pivots, key);
+        Keys.LargestLteSubsequence(oldindex.pivots, key, 0, |leftindex.pivots|);
         assert oldindex.children[llte+1] == leftindex.children[llte+1];
       } else {
         AllKeysIsConsistentWithInterpretation(rightindex, key);
         var llte := Keys.LargestLte(rightindex.pivots, key);
+        Keys.LargestLteSubsequence(oldindex.pivots, key, |leftindex.pivots|+1, |oldindex.pivots|);
         assert oldindex.children[|leftindex.children| + llte + 1] == rightindex.children[llte+1];
       }
     }
@@ -203,8 +238,24 @@ abstract module BtreeSpec {
     || SplitIndex(oldnode, leftnode, rightnode, pivot)
   }
 
+  lemma SplitNodePreservesWF(oldnode: Node, leftnode: Node, rightnode: Node, pivot: Key)
+    requires WF(oldnode)
+    requires SplitNode(oldnode, leftnode, rightnode, pivot)
+    ensures WF(leftnode)
+    ensures WF(rightnode)
+  {
+    if SplitLeaf(oldnode, leftnode, rightnode, pivot) {
+      SplitLeafPreservesWF(oldnode, leftnode, rightnode, pivot);
+    } else {
+      SplitIndexPreservesWF(oldnode, leftnode, rightnode, pivot);
+    }
+  }
+    
   lemma SplitNodeInterpretation(oldnode: Node, leftnode: Node, rightnode: Node, pivot: Key)
     requires SplitNode(oldnode, leftnode, rightnode, pivot)
+    requires WF(oldnode)
+    requires WF(leftnode)
+    requires WF(rightnode)
     ensures Interpretation(oldnode) == Keys.MapPivotedUnion(Interpretation(leftnode), pivot, Interpretation(rightnode))
   {
     if SplitLeaf(oldnode, leftnode, rightnode, pivot) {
@@ -233,13 +284,48 @@ abstract module BtreeSpec {
       }
     }
   }
+
+  lemma SplitNodePotentialPivots(oldnode: Node, leftnode: Node, rightnode: Node, pivot: Key)
+    requires WF(oldnode)
+    requires SplitNode(oldnode, leftnode, rightnode, pivot)
+    ensures PotentialPivots(leftnode) <= PotentialPivots(oldnode)
+    ensures PotentialPivots(rightnode) <= PotentialPivots(oldnode)
+    ensures forall key :: key in PotentialPivots(leftnode) ==> Keys.lt(key, pivot)
+    ensures forall key :: key in PotentialPivots(rightnode) ==> Keys.lt(pivot, key)
+  {
+    forall key | key in PotentialPivots(leftnode)
+      ensures key in PotentialPivots(oldnode)
+      ensures Keys.lt(key, pivot)
+    {
+      if oldnode.Leaf? {
+        var i :| 0 < i < |leftnode.keys| && key == leftnode.keys[i];
+        assert oldnode.keys[i] == key;
+        Keys.IsStrictlySortedImpliesLt(oldnode.keys, i, |leftnode.keys|);
+      } else {
+        var i :| 0 <= i < |leftnode.pivots| && key == leftnode.pivots[i];
+        Keys.IsStrictlySortedImpliesLt(oldnode.pivots, i, |leftnode.pivots|);        
+      }
+    }
+    forall key | key in PotentialPivots(rightnode)
+      ensures key in PotentialPivots(oldnode)
+      ensures Keys.lt(pivot, key)
+    {
+      if oldnode.Leaf? {
+        var i :| 0 < i < |rightnode.keys| && key == rightnode.keys[i];
+        assert oldnode.keys[|leftnode.keys| + i] == key;
+        Keys.IsStrictlySortedImpliesLt(oldnode.keys, |leftnode.keys|, |leftnode.keys| + i);
+      } else {
+        var i :| 0 <= i < |rightnode.pivots| && key == rightnode.pivots[i];
+        Keys.IsStrictlySortedImpliesLt(oldnode.pivots, |leftnode.pivots|, |leftnode.pivots| + i + 1);
+      }
+    }
+  }
   
   predicate SplitChildOfIndex(oldindex: Node, newindex: Node, childidx: int)
   {
     && oldindex.Index?
     && newindex.Index?
     && WF(oldindex)
-    && WF(newindex)
     && 0 <= childidx < |oldindex.children|
     && |newindex.children| == |oldindex.children| + 1 // FIXME: WTF?  Dafny can't get these from WF?
     && |newindex.pivots| == |oldindex.pivots| + 1
@@ -247,15 +333,70 @@ abstract module BtreeSpec {
     && SplitNode(oldindex.children[childidx], newindex.children[childidx], newindex.children[childidx+1], newindex.pivots[childidx])
     && newindex.pivots == Seq.insert(oldindex.pivots, newindex.pivots[childidx], childidx)
     && newindex.children == Seq.replace1with2(oldindex.children, newindex.children[childidx], newindex.children[childidx+1], childidx)
-    //oldindex.children[..childidx] + [newindex.children[childidx], newindex.children[childidx+1]] + oldindex.children[childidx+1..]
   }
 
+  lemma SplitChildOfIndexPreservesWF(oldindex: Node, newindex: Node, childidx: int)
+    requires WF(oldindex)
+    requires SplitChildOfIndex(oldindex, newindex, childidx)
+    ensures WF(newindex)
+  {
+    var pivot := newindex.pivots[childidx];
+    
+    if oldindex.children[childidx].Leaf? {
+      assert pivot == oldindex.children[childidx].keys[|newindex.children[childidx].keys|];
+      assert pivot in PotentialPivots(oldindex.children[childidx]);
+    } else {
+      assert pivot in PotentialPivots(oldindex.children[childidx]);
+    }
+    Keys.strictlySortedInsert2(oldindex.pivots, pivot, childidx);
+
+    forall i | 0 <= i < |newindex.children|
+      ensures WF(newindex.children[i])
+    {
+      if i < childidx {
+      } else if i == childidx {
+        SplitNodePreservesWF(oldindex.children[childidx], newindex.children[childidx], newindex.children[childidx+1], pivot);
+      } else if i == childidx + 1 {
+        SplitNodePreservesWF(oldindex.children[childidx], newindex.children[childidx], newindex.children[childidx+1], pivot);
+      } else {
+        assert newindex.children[i] == oldindex.children[i-1];
+      }
+    }
+
+    forall i, key | 0 <= i < |newindex.children| - 1 && key in PotentialPivots(newindex.children[i])
+      ensures Keys.lt(key, newindex.pivots[i])
+    {
+      if i < childidx {
+      } else if i == childidx {
+        SplitNodePotentialPivots(oldindex.children[childidx], newindex.children[childidx], newindex.children[childidx+1], pivot);
+      } else if i == childidx + 1 {
+        SplitNodePotentialPivots(oldindex.children[childidx], newindex.children[childidx], newindex.children[childidx+1], pivot);
+      } else {
+        assert newindex.children[i] == oldindex.children[i-1];
+      }      
+    }
+    
+    forall i, key | 0 < i < |newindex.children| && key in PotentialPivots(newindex.children[i])
+      ensures Keys.lt(newindex.pivots[i-1], key)
+    {
+      if i < childidx {
+      } else if i == childidx {
+        SplitNodePotentialPivots(oldindex.children[childidx], newindex.children[childidx], newindex.children[childidx+1], pivot);
+      } else if i == childidx + 1 {
+        SplitNodePotentialPivots(oldindex.children[childidx], newindex.children[childidx], newindex.children[childidx+1], pivot);
+      } else {
+        assert newindex.children[i] == oldindex.children[i-1];
+      }      
+    }
+    
+  }
+  
   lemma SplitChildOfIndexPreservesAllKeys(oldindex: Node, newindex: Node, childidx: int)
     requires SplitChildOfIndex(oldindex, newindex, childidx)
     ensures AllKeys(newindex) == AllKeys(oldindex)
   {
     assert WF(oldindex);
-    assert WF(newindex);
+    SplitChildOfIndexPreservesWF(oldindex, newindex, childidx);
     
     forall key | key in AllKeys(oldindex)
       ensures key in AllKeys(newindex)
@@ -286,6 +427,7 @@ abstract module BtreeSpec {
   
   lemma SplitChildOfIndexPreservesInterpretation(oldindex: Node, newindex: Node, childidx: int)
     requires SplitChildOfIndex(oldindex, newindex, childidx)
+    requires WF(newindex);
     ensures Interpretation(newindex) == Interpretation(oldindex)
   {
     var newint := Interpretation(newindex);
@@ -309,11 +451,21 @@ abstract module BtreeSpec {
     {
       var llte := Keys.LargestLte(oldindex.pivots, key);
       if llte + 1 < childidx {
-        assert llte == Keys.LargestLte(newindex.pivots, key);
+        Keys.LargestLteIsUnique2(newindex.pivots, key, llte);
+        // assert key in newint && newint[key] == oldint[key];
       } else if llte + 1 == childidx {
+        if Keys.lt(key, pivot) {
+          Keys.LargestLteIsUnique2(newindex.pivots, key, llte);
+        } else {
+          assert llte+2 < |newindex.pivots| ==> newindex.pivots[llte+2] == oldindex.pivots[llte+1];
+          Keys.LargestLteIsUnique2(newindex.pivots, key, llte+1);
+        }
       } else {
         var newllte := llte + 1;
-        assert newllte == Keys.LargestLte(newindex.pivots, key);
+        assert newindex.pivots[newllte] == oldindex.pivots[llte];
+        assert newllte+1 < |newindex.pivots| ==> newindex.pivots[newllte+1] == oldindex.pivots[llte+1];
+        assert newllte+1 < |newindex.pivots| ==> Keys.lt(key, newindex.pivots[newllte+1]);
+        Keys.LargestLteIsUnique2(newindex.pivots, key, newllte);
         assert newindex.children[newllte+1] == oldindex.children[llte+1];
       }
     }
@@ -323,17 +475,16 @@ abstract module BtreeSpec {
     {
       var llte := Keys.LargestLte(newindex.pivots, key);
       if llte + 1 < childidx {
-        assert llte == Keys.LargestLte(oldindex.pivots, key);
+        Keys.LargestLteIsUnique2(oldindex.pivots, key, llte);
       } else if llte + 1 == childidx {
-        var oldllte := llte;
-        assert oldllte == Keys.LargestLte(oldindex.pivots, key);
-        assert key in Interpretation(oldindex.children[Keys.LargestLte(oldindex.pivots, key) + 1]);
+        Keys.LargestLteIsUnique2(oldindex.pivots, key, llte);
       } else if llte + 1 == childidx + 1 {
         var oldllte := llte - 1;
+        Keys.LargestLteIsUnique2(oldindex.pivots, key, oldllte);
         assert oldllte == Keys.LargestLte(oldindex.pivots, key);
         assert key in Interpretation(oldindex.children[Keys.LargestLte(oldindex.pivots, key) + 1]);
       } else {
-        assert llte - 1 == Keys.LargestLte(oldindex.pivots, key);
+        Keys.LargestLteIsUnique2(oldindex.pivots, key, llte-1);
       }
     }
   }
@@ -352,12 +503,12 @@ abstract module BtreeSpec {
       Leaf(Seq.insert(leaf.keys, key, llte+1), Seq.insert(leaf.values, value, llte+1))
   }
 
-  lemma InsertLeafIsCorrect(leaf: Node, key: Key, value: Value, result: Node)
+  lemma InsertLeafIsCorrect(leaf: Node, key: Key, value: Value)
     requires leaf.Leaf?
     requires WF(leaf)
-    requires result == InsertLeaf(leaf, key, value)
-    ensures Interpretation(result) == Interpretation(leaf)[key := value]
+    ensures Interpretation(InsertLeaf(leaf, key, value)) == Interpretation(leaf)[key := value]
   {
+    var result := InsertLeaf(leaf, key, value);
     var llte := Keys.LargestLte(leaf.keys, key);
     if 0 <= llte && leaf.keys[llte] == key {
       assert Interpretation(result) == Interpretation(leaf)[key := value];
